HoG/Invariant/Hamiltonian/SatEncoding.lean
@@ -1,261 +1,338 @@
-import Mathlib.Data.Matrix.Basic
-
-import HoG.Tactic
 import HoG.Graph
 import HoG.Walk
 import HoG.Invariant.ConnectedComponents
 import HoG.Invariant.Hamiltonian.Definition
+
 import LeanSAT
 
 namespace HoG
 
-open LeanSAT
+open LeanSAT Encode VEncCNF
 
-/--
-  For a given graph `g` encode finding a Hamiltonian path as a SAT problem.
--/
-def Graph.hamiltonianPathEncodeToSAT (g : Graph) :
-  Encode.EncCNF (Fin g.vertexSize → Fin g.vertexSize → IVar) :=
-  open Encode.EncCNF in do
-  let n := g.vertexSize
-  if H : 0 < n then
-    let varArr ←
-      Array.initM n fun i =>
-        Array.initM n fun j =>
-          mkVar s!"x_{i},{j}"
-    -- xᵢ,ⱼ represents vertex i appearing on the path at position j, as i,j ∈ {1,…,n}
-    let vertexAtLoc (i : Fin n) (j : Fin n) := (varArr[i]!)[j]!
-    -- ⋀ᵢ (⋁ⱼ (xᵢ,ⱼ)) ↔ every vertex appears somewhere on the path
-    for i in List.fins n do
-      let vars := (List.fins n).map (vertexAtLoc i) |>.toArray
-      addClause (vars.map LitVar.mkPos)
-    -- ⋀ᵢ (⋁ⱼ (xⱼ,ᵢ)) ↔ every position on the path is occupied by some vertex
-    for i in List.fins n do
-      let vars := (List.fins n).map (fun j => vertexAtLoc j i) |>.toArray
-      addClause (vars.map LitVar.mkPos)
-    -- ⋀_i ⋀_j≠k (¬xᵢ,ⱼ ∨ ¬xᵢ,ₖ) ↔ no vertex appears on the path more than once
-    for i in List.fins n do
-      for j in List.fins n do
-        for k in List.fins n do
-          if j ≠ k then
-            let clause := #[(vertexAtLoc i j), (vertexAtLoc i k)].map LitVar.mkNeg
-            addClause clause
-    -- ⋀_i ⋀_j≠k (¬xⱼ,ᵢ ∨ ¬xₖ,ᵢ) ↔ no distinct vertices occupy the same position on the path
-    for i in List.fins n do
-      for j in List.fins n do
-        for k in List.fins n do
-          if j ≠ k then
-            let clause := #[vertexAtLoc j i, vertexAtLoc k i].map LitVar.mkNeg
-            addClause clause
-    -- ⋀_(k < n) ⋀_((i,j) ∉ E) (¬xₖ,ᵢ ∨ ¬xₖ₊₁,ⱼ) ↔ non-adjacent vertices cannot be adjacent on the path
-    for k in List.fins n do
-      if k < n-1 then
-        for i in List.fins n do
-          for j in List.fins i do
-            if (Edge.mk i j) ∉ g.edgeTree then
-              let next : Fin n := ⟨ (k + 1) % n, by apply Nat.mod_lt; exact H⟩ -- TODO: hack, make nicer
-              let clause := #[vertexAtLoc k i, vertexAtLoc next i].map LitVar.mkNeg
-              addClause clause
+/-- (Var i j = true) means: "at position j on the path is vertex i". -/
+structure Var (n : Nat) where
+  vertex : Fin n
+  pos : Fin n
+deriving DecidableEq
 
-    return vertexAtLoc
-  else
-    have h' : g.vertexSize = 0 := by simp_all
-    return (by rw [h']; intro x; have := Fin.isLt x; contradiction)
+instance {g : Graph} :  MyFinEnum.FinEnum (Var g.vertexSize) := .ofEquiv {
+  toFun := fun {vertex,pos} => (vertex,pos)
+  invFun := fun (vertex,pos) => {vertex,pos}
+  left_inv := by intro; simp
+  right_inv := by intro; simp
+}
 
-/--
-  For a given graph `g` encode finding a Hamiltonian cycle as a SAT problem.
--/
-def Graph.hamiltonianCycleEncodeToSAT (g : Graph) :
-  Encode.EncCNF (Fin g.vertexSize → Fin (g.vertexSize + 1) → IVar) :=
-  open Encode.EncCNF in do
-  let n := g.vertexSize
-  if H : 0 < n then
-    let varArr ←
-      Array.initM n fun i =>
-        Array.initM (n+1) fun j =>
-          mkVar s!"x_{i},{j}"
-    -- xᵢ,ⱼ represents vertex i appearing on the path at position j
-    -- i ranges from 1 to n, j ranges from 1 to n+1 (as it needs to return to the first vertex)
-    let vertexAtLoc (i : Fin n) (j : Fin (n + 1)) := (varArr[i]!)[j]!
-    -- The cycle starts and end at vertex 0
-    addClause #[LitVar.mkPos (vertexAtLoc ⟨0, H⟩ ⟨0, by simp [H]⟩)]
-    addClause #[LitVar.mkPos (vertexAtLoc ⟨0, H⟩ n)]
-    -- ⋀ᵢ (⋁ⱼ (xᵢ,ⱼ)) ↔ every vertex appears somewhere on the path
-    -- we don't need to consider the last position of the path
-    for i in List.fins n do
-      let vars := (List.fins n).map (vertexAtLoc i) |>.toArray
-      addClause (vars.map LitVar.mkPos)
-    -- ⋀ᵢ (⋁ⱼ (xⱼ,ᵢ)) ↔ every position on the path is occupied by some vertex
-    for i in List.fins n do
-      let vars := (List.fins n).map (fun j => vertexAtLoc j i) |>.toArray
-      addClause (vars.map LitVar.mkPos)
-    -- ⋀_i ⋀_j≠k (¬xᵢ,ⱼ ∨ ¬xᵢ,ₖ) ↔ no vertex appears on the path more than once
-    -- except vertex 0 on the first and last place
-    for i in List.fins n do
-      for j in List.fins n do
-        for k in List.fins n do
-          if j ≠ k then
-            let clause := #[(vertexAtLoc i j), (vertexAtLoc i k)].map LitVar.mkNeg
-            addClause clause
-    -- ⋀_i ⋀_j≠k (¬xⱼ,ᵢ ∨ ¬xₖ,ᵢ) ↔ no distinct vertices occupy the same position on the path
-    for i in List.fins (n + 1) do
-      for j in List.fins n do
-        for k in List.fins n do
-          if j ≠ k then
-            let clause := #[vertexAtLoc j i, vertexAtLoc k i].map LitVar.mkNeg
-            addClause clause
-    -- ⋀_(k < n) ⋀_((i,j) ∉ E) (¬xₖ,ᵢ ∨ ¬xₖ₊₁,ⱼ) ↔ non-adjacent vertices cannot be adjacent on the path
-    for k in List.fins n do
-      if k < n-1 then
-        for i in List.fins n do
-          for j in List.fins i do
-            if (Edge.mk i j) ∉ g.edgeTree then
-              let next : Fin n := ⟨ (k + 1) % n, by apply Nat.mod_lt; exact H⟩ -- TODO: hack, make nicer
-              let clause := #[vertexAtLoc k i, vertexAtLoc next i].map LitVar.mkNeg
-              addClause clause
-    return vertexAtLoc
-  else
-    have h' : g.vertexSize = 0 := by simp_all
-    return (by rw [h']; intro x; have := Fin.isLt x; contradiction)
+def verticesAtPosition {n : Nat} (j : Fin n) : List (Literal <| Var n) :=
+  List.finRange n |>.map (Literal.pos <| Var.mk · j)
 
-/--
-  Given a list of vertices of a graph, try to construct a `Path` in the graph from them.
-  If the construction fails, return `none`.
--/
-def buildPath {g : Graph} : Option (List (g.vertex)) → Option ((u v : g.vertex) ×' Path g u v)
-  | none => none
-  | some [] => none
-  | some (v :: vs) =>
-    let rec fold (first last : g.vertex) (p : Path g first last) :
-      List (g.vertex) → Option ((u v : g.vertex) ×' Path g u v)
-    | [] => some ⟨first, last, p⟩
-    | v :: vs =>
-      if h : g.adjacent last v then
-        let w := Walk.right p.walk h
-        if h' : Walk.isPath w = true then
-          fold first v ⟨w, h'⟩ vs
-        else
-          none
-      else
-        none
-    fold v v (Path.trivialPath v) vs
+def vertexAtPositions {n : Nat} (i : Fin n) : List (Literal <| Var n) :=
+  List.finRange n |>.map (Literal.pos <| Var.mk i ·)
 
-/--
-  Given a list of vertices of a graph, try to construct a `Cycle` in the graph from them.
-  If the construction fails, return `none`.
--/
-def buildCycle {g : Graph} : Option (List (g.vertex)) → Option ((u : g.vertex) ×' Cycle g u)
-  | none => none
-  | some [] => none
-  | some [v] =>
-    let walk := Walk.trivial v
-    some ⟨v, walk, by simp [List.all_distinct, Walk.vertices]⟩
-  | some (v₁ :: v₂ :: vs) =>
-    let rec fold (first last : g.vertex) (p : Path g first last) :
-      List (g.vertex) → Option ((u v : g.vertex) ×' Path g u v)
-    | [] => some ⟨first, last, p⟩
-    | v :: vs =>
-      if h : g.adjacent last v then
-        let w := Walk.right p.walk h
-        if h' : Walk.isPath w = true then
-          fold first v ⟨w, h'⟩ vs
-        else
-          none
-      else
-        none
-    let path := fold v₂ v₂ (Path.trivialPath v₂) vs
-    match path with
-    | none => none
-    | some ⟨u,v,p⟩ =>
-      if h : u = v₂ ∧ v = v₁ ∧ g.adjacent v₁ v₂ then
-        have u_eq_v₂ := h.1
-        have v_eq_v₁ := h.2.1
-        let w : ClosedWalk g v₁ := Walk.left h.2.2 (u_eq_v₂ ▸ v_eq_v₁ ▸ p.walk)
-        if cyc : w.isCycle then
-        some ⟨ v₁,
-          { cycle := w,
-            isCycle := by
-              subst u_eq_v₂
-              subst v_eq_v₁
-              exact cyc
-          }⟩
-        else
-          none
-      else
-        none
+def encoding1 (g : Graph) : VEncCNF (Literal (Var g.vertexSize)) Unit (fun τ =>
+    (∀ i, ∃ j, τ (Var.mk i j)) ∧
+    (∀ i, atMost 1 (Multiset.ofList <| vertexAtPositions i) τ) ∧
+    (∀ j, ∃ i, τ (Var.mk i j)) ∧
+    (∀ j, atMost 1 (Multiset.ofList <| verticesAtPosition j) τ)
+  ) :=
+  seq[
+    for_all (List.toArray <| List.finRange g.vertexSize) fun i =>
+      addClause (List.toArray (vertexAtPositions i)),
+    for_all (List.toArray <| List.finRange g.vertexSize) fun i =>
+      amoPairwise (List.toArray (vertexAtPositions i)),
+    for_all (List.toArray <| List.finRange g.vertexSize) fun j =>
+      addClause (List.toArray (verticesAtPosition j)),
+    for_all (List.toArray <| List.finRange g.vertexSize) fun j =>
+      amoPairwise (List.toArray (verticesAtPosition j))
+  ]
+  |>.mapProp (by
+    ext τ
+    simp [vertexAtPositions, verticesAtPosition, Clause.satisfies_iff, LitVar.satisfies_iff,
+          LitVar.toVar, LitVar.polarity]
+  )
 
-/--
-  Given a graph `g`, encode the problem of finding a Hamiltonian path as a SAT
-  problem and then from the solution construct a `HamiltonianPath` in the graph.
--/
-def findHamiltonianPath [Solver IO] (g : Graph) :
-  IO (Option ((u v : g.vertex) ×' HamiltonianPath u v)) := do
-  let (vertexAtLoc, enc) := Encode.EncCNF.new! (g.hamiltonianPathEncodeToSAT)
+def encoding2 (g : Graph) : VEncCNF (Literal (Var g.vertexSize)) Unit (fun τ =>
+    (∀ k k', k.val + 1 =  k'.val →
+      ∀ i j, ¬ g.badjacent i j → ¬ (τ (Var.mk i k)) ∨ ¬ (τ (Var.mk j k'))
+    )
+  ) :=
+  seq[
+    for_all (List.toArray <| List.finRange g.vertexSize) (fun k =>
+    for_all (List.toArray <| List.finRange g.vertexSize) fun k' =>
+      guard (k.val + 1 = k'.val) (fun h =>
+        for_all (List.toArray <| List.finRange g.vertexSize) fun i =>
+        for_all (List.toArray <| List.finRange g.vertexSize) fun j =>
+          guard (¬g.badjacent i j) (fun h' =>
+            addClause (#[Var.mk i k, Var.mk j k'].map LitVar.mkNeg)
+          )
+      )
+    )
+  ]
+  |>.mapProp (by
+    ext τ
+    apply Iff.intro
+    · intros h k k' seq i j adj
+      simp_all [vertexAtPositions, verticesAtPosition, Clause.satisfies_iff, LitVar.satisfies_iff,
+            LitVar.toVar, LitVar.polarity, LitVar.mkNeg, not_false_eq_true, implies_true, and_self,
+            LitVar.mkPos_or_mkNeg
+      ]
+      have := h k k'
+      simp [seq] at this
+      have foo := this i j
+      simp [adj] at foo
+      let ⟨l, cond⟩ := foo
+      unhygienic with_reducible aesop_destruct_products
+      unhygienic aesop_cases left <;> [(unhygienic aesop_cases left_1); (unhygienic aesop_cases left_1)]
+      · aesop_subst [h_1, h_2]
+        simp_all only [true_or]
+      · aesop_subst [h_1, h_2]
+        simp_all only [or_self]
+      · aesop_subst [h_2, h_1]
+        simp_all only [or_self]
+      · aesop_subst [h_2, h_1]
+        simp_all only [or_true]
+    · intros h
+      simp_all [vertexAtPositions, verticesAtPosition, Clause.satisfies_iff, LitVar.satisfies_iff,
+            LitVar.toVar, LitVar.polarity, LitVar.mkNeg, not_false_eq_true, implies_true, and_self,
+            LitVar.mkPos_or_mkNeg
+      ]
+      intros k k'
+      have := h k k'
+      have foo : k.val + 1 ≠ k'.val ∨ k.val + 1 = k'.val := by apply Or.symm; apply Decidable.em
+      cases' foo with neq eq
+      simp [neq]
+      simp [eq]
+      intros i j
+      have moo : g.badjacent i j ∨ ¬ g.badjacent i j := by apply Decidable.em
+      cases' moo with adj nadj
+      simp [adj]
+      simp [nadj]
+      simp at nadj
+      have bar := this eq i j nadj
+      cases' bar with l r
+      · simp_all only [implies_true, forall_true_left]
+        apply Exists.intro
+        apply And.intro
+        apply Or.inl
+        apply Eq.refl
+        simp_all only
+      · simp_all only [implies_true, forall_true_left]
+        apply Exists.intro
+        apply And.intro
+        apply Or.inr
+        apply Eq.refl
+        simp_all only
+  )
+
+def my_enc (g : Graph) := seq (encoding1 g) (encoding2 g)
+
+def showNoHamiltonianPath [Solver IO] (g : Graph) :
+  -- IO (Option ((g : Graph) ×' (¬ ∃ (u v : g.vertex) (p : Path g u v), p.isHamiltonian))) := do
+  IO Unit := do
+  let enc := my_enc g
+  let cnf := enc.val.toICnf
   -- IO.println s!"{enc}"
-  match ← Solver.solve enc.toFormula with
+  match ← Solver.solve cnf with
   | .error =>
     IO.println "error"
-    return none
   | .unsat =>
     IO.println "unsat"
-    return none
-  | .sat assn =>
-    if h : 0 < g.vertexSize then
-      let mut path : Array (g.vertex) := Array.mkArray g.vertexSize ⟨0, h⟩
-      for i in List.fins g.vertexSize do
-        for j in List.fins g.vertexSize do
-          match assn.find? (vertexAtLoc i j) with
-          | none => panic! "wtf"
-          | some true =>
-            path := path.set! j i
-          | some false =>
-            path := path
-      let p := (buildPath (some path.toList))
-      match p with
-      | none => return none
-      | some ⟨u,v,p⟩ =>
-        if h' : p.isHamiltonian then
-          return some ⟨u,v,p,h'⟩
-        else
-          return none
-    else
-      return none
+  | .sat _ =>
+    return ()
 
-/--
-  Given a graph `g`, encode the problem of finding a Hamiltonian cycle as a SAT
-  problem and then from the solution construct a `HamiltonianCycle` in the graph.
--/
-def findHamiltonianCycle [Solver IO] (g : Graph) :
-  IO (Option ((u : g.vertex) ×' HamiltonianCycle g u)) := do
-  let (vertexAtLoc, enc) := Encode.EncCNF.new! (g.hamiltonianCycleEncodeToSAT)
-  match ← Solver.solve enc.toFormula with
-  | .error =>
-    IO.println "error"
-    return none
-  | .unsat =>
-    IO.println "unsat"
-    return none
-  | .sat assn =>
-    if h : 0 < g.vertexSize then
-      let mut path : Array (g.vertex) := Array.mkArray (g.vertexSize + 1) ⟨0, by simp [h]⟩
-      for i in List.fins g.vertexSize do
-        for j in List.fins (g.vertexSize + 1) do
-          let v := vertexAtLoc i j
-          match assn.find? v with
-          | none => panic! s!"no assignment for ({i}, {j}) → {v}"
-          | some true =>
-            path := path.set! j i
-          | some false =>
-            path := path
-      let c := (buildCycle (some path.toList))
-      match c with
-      | none => return none
-      | some ⟨u,c⟩ =>
-        if h' : c.isHamiltonian then
-          return some ⟨u, c, h'⟩
-        else
-          return none
-    else
-      return none
+-- /--
+--   For a given graph `g` encode finding a Hamiltonian cycle as a SAT problem.
+-- -/
+-- def Graph.hamiltonianCycleEncodeToSAT (g : Graph) :
+--   Encode.EncCNF (Fin g.vertexSize → Fin (g.vertexSize + 1) → IVar) :=
+--   open Encode.EncCNF in do
+--   let n := g.vertexSize
+--   if H : 0 < n then
+--     let varArr ←
+--       Array.initM n fun i =>
+--         Array.initM (n+1) fun j =>
+--           mkVar s!"x_{i},{j}"
+--     -- xᵢ,ⱼ represents vertex i appearing on the path at position j
+--     -- i ranges from 1 to n, j ranges from 1 to n+1 (as it needs to return to the first vertex)
+--     let vertexAtLoc (i : Fin n) (j : Fin (n + 1)) := (varArr[i]!)[j]!
+--     -- The cycle starts and end at vertex 0
+--     addClause #[LitVar.mkPos (vertexAtLoc ⟨0, H⟩ ⟨0, by simp [H]⟩)]
+--     addClause #[LitVar.mkPos (vertexAtLoc ⟨0, H⟩ n)]
+--     -- ⋀ᵢ (⋁ⱼ (xᵢ,ⱼ)) ↔ every vertex appears somewhere on the path
+--     -- we don't need to consider the last position of the path
+--     for i in List.fins n do
+--       let vars := (List.fins n).map (vertexAtLoc i) |>.toArray
+--       addClause (vars.map LitVar.mkPos)
+--     -- ⋀ᵢ (⋁ⱼ (xⱼ,ᵢ)) ↔ every position on the path is occupied by some vertex
+--     for i in List.fins n do
+--       let vars := (List.fins n).map (fun j => vertexAtLoc j i) |>.toArray
+--       addClause (vars.map LitVar.mkPos)
+--     -- ⋀_i ⋀_j≠k (¬xᵢ,ⱼ ∨ ¬xᵢ,ₖ) ↔ no vertex appears on the path more than once
+--     -- except vertex 0 on the first and last place
+--     for i in List.fins n do
+--       for j in List.fins n do
+--         for k in List.fins n do
+--           if j ≠ k then
+--             let clause := #[(vertexAtLoc i j), (vertexAtLoc i k)].map LitVar.mkNeg
+--             addClause clause
+--     -- ⋀_i ⋀_j≠k (¬xⱼ,ᵢ ∨ ¬xₖ,ᵢ) ↔ no distinct vertices occupy the same position on the path
+--     for i in List.fins (n + 1) do
+--       for j in List.fins n do
+--         for k in List.fins n do
+--           if j ≠ k then
+--             let clause := #[vertexAtLoc j i, vertexAtLoc k i].map LitVar.mkNeg
+--             addClause clause
+--     -- ⋀_(k < n) ⋀_((i,j) ∉ E) (¬xₖ,ᵢ ∨ ¬xₖ₊₁,ⱼ) ↔ non-adjacent vertices cannot be adjacent on the path
+--     for k in List.fins n do
+--       if k < n-1 then
+--         for i in List.fins n do
+--           for j in List.fins i do
+--             if (Edge.mk i j) ∉ g.edgeTree then
+--               let next : Fin n := ⟨ (k + 1) % n, by apply Nat.mod_lt; exact H⟩ -- TODO: hack, make nicer
+--               let clause := #[vertexAtLoc k i, vertexAtLoc next i].map LitVar.mkNeg
+--               addClause clause
+--     return vertexAtLoc
+--   else
+--     have h' : g.vertexSize = 0 := by simp_all
+--     return (by rw [h']; intro x; have := Fin.isLt x; contradiction)
+
+-- /--
+--   Given a list of vertices of a graph, try to construct a `Path` in the graph from them.
+--   If the construction fails, return `none`.
+-- -/
+-- def buildPath {g : Graph} : Option (List (g.vertex)) → Option ((u v : g.vertex) ×' Path g u v)
+--   | none => none
+--   | some [] => none
+--   | some (v :: vs) =>
+--     let rec fold (first last : g.vertex) (p : Path g first last) :
+--       List (g.vertex) → Option ((u v : g.vertex) ×' Path g u v)
+--     | [] => some ⟨first, last, p⟩
+--     | v :: vs =>
+--       if h : g.adjacent last v then
+--         let w := Walk.right p.walk h
+--         if h' : Walk.isPath w = true then
+--           fold first v ⟨w, h'⟩ vs
+--         else
+--           none
+--       else
+--         none
+--     fold v v (Path.trivialPath v) vs
+
+-- /--
+--   Given a list of vertices of a graph, try to construct a `Cycle` in the graph from them.
+--   If the construction fails, return `none`.
+-- -/
+-- def buildCycle {g : Graph} : Option (List (g.vertex)) → Option ((u : g.vertex) ×' Cycle g u)
+--   | none => none
+--   | some [] => none
+--   | some [v] =>
+--     let walk := Walk.trivial v
+--     some ⟨v, walk, by simp [List.all_distinct, Walk.vertices]⟩
+--   | some (v₁ :: v₂ :: vs) =>
+--     let rec fold (first last : g.vertex) (p : Path g first last) :
+--       List (g.vertex) → Option ((u v : g.vertex) ×' Path g u v)
+--     | [] => some ⟨first, last, p⟩
+--     | v :: vs =>
+--       if h : g.adjacent last v then
+--         let w := Walk.right p.walk h
+--         if h' : Walk.isPath w = true then
+--           fold first v ⟨w, h'⟩ vs
+--         else
+--           none
+--       else
+--         none
+--     let path := fold v₂ v₂ (Path.trivialPath v₂) vs
+--     match path with
+--     | none => none
+--     | some ⟨u,v,p⟩ =>
+--       if h : u = v₂ ∧ v = v₁ ∧ g.adjacent v₁ v₂ then
+--         have u_eq_v₂ := h.1
+--         have v_eq_v₁ := h.2.1
+--         let w : ClosedWalk g v₁ := Walk.left h.2.2 (u_eq_v₂ ▸ v_eq_v₁ ▸ p.walk)
+--         if cyc : w.isCycle then
+--         some ⟨ v₁,
+--           { cycle := w,
+--             isCycle := by
+--               subst u_eq_v₂
+--               subst v_eq_v₁
+--               exact cyc
+--           }⟩
+--         else
+--           none
+--       else
+--         none
+
+-- /--
+--   Given a graph `g`, encode the problem of finding a Hamiltonian path as a SAT
+--   problem and then from the solution construct a `HamiltonianPath` in the graph.
+-- -/
+-- def findHamiltonianPath [Solver IO] (g : Graph) :
+--   IO (Option ((u v : g.vertex) ×' HamiltonianPath u v)) := do
+--   let (vertexAtLoc, enc) := Encode.EncCNF.new! (g.hamiltonianPathEncodeToSAT)
+--   -- IO.println s!"{enc}"
+--   match ← Solver.solve enc.toFormula with
+--   | .error =>
+--     IO.println "error"
+--     return none
+--   | .unsat =>
+--     IO.println "unsat"
+--     return none
+--   | .sat assn =>
+--     if h : 0 < g.vertexSize then
+--       let mut path : Array (g.vertex) := Array.mkArray g.vertexSize ⟨0, h⟩
+--       for i in List.fins g.vertexSize do
+--         for j in List.fins g.vertexSize do
+--           match assn.find? (vertexAtLoc i j) with
+--           | none => panic! "wtf"
+--           | some true =>
+--             path := path.set! j i
+--           | some false =>
+--             path := path
+--       let p := (buildPath (some path.toList))
+--       match p with
+--       | none => return none
+--       | some ⟨u,v,p⟩ =>
+--         if h' : p.isHamiltonian then
+--           return some ⟨u,v,p,h'⟩
+--         else
+--           return none
+--     else
+--       return none
+
+-- /--
+--   Given a graph `g`, encode the problem of finding a Hamiltonian cycle as a SAT
+--   problem and then from the solution construct a `HamiltonianCycle` in the graph.
+-- -/
+-- def findHamiltonianCycle [Solver IO] (g : Graph) :
+--   IO (Option ((u : g.vertex) ×' HamiltonianCycle g u)) := do
+--   let (vertexAtLoc, enc) := Encode.EncCNF.new! (g.hamiltonianCycleEncodeToSAT)
+--   match ← Solver.solve enc.toFormula with
+--   | .error =>
+--     IO.println "error"
+--     return none
+--   | .unsat =>
+--     IO.println "unsat"
+--     return none
+--   | .sat assn =>
+--     if h : 0 < g.vertexSize then
+--       let mut path : Array (g.vertex) := Array.mkArray (g.vertexSize + 1) ⟨0, by simp [h]⟩
+--       for i in List.fins g.vertexSize do
+--         for j in List.fins (g.vertexSize + 1) do
+--           let v := vertexAtLoc i j
+--           match assn.find? v with
+--           | none => panic! s!"no assignment for ({i}, {j}) → {v}"
+--           | some true =>
+--             path := path.set! j i
+--           | some false =>
+--             path := path
+--       let c := (buildCycle (some path.toList))
+--       match c with
+--       | none => return none
+--       | some ⟨u,c⟩ =>
+--         if h' : c.isHamiltonian then
+--           return some ⟨u, c, h'⟩
+--         else
+--           return none
+--     else
+--       return none
 
 end HoG
