lakefile.lean
@@ -9,7 +9,7 @@ require mathlib from git
   "https://github.com/leanprover-community/mathlib4.git" @ "v4.5.0"
 
 require «lean-sat» from git
-  "https://github.com/JamesGallicchio/LeanSAT.git" @ "dev"
+  "https://github.com/cilinder/LeanSAT.git" @ "alt"
 
 @[default_target]
 lean_lib HoG
